Fixed some issues related to IMM fairness in finite graphs; moved some ImmFair parts to other files

src/imm/ImmFair.v
@@ -1,162 +1,15 @@
 Require Import Events.
 Require Import Execution.
 Require Import Execution_eco.
-Require Import imm_s imm_s_ppo imm_s_hb imm_s_rfppo.
-Require Import imm_hb imm_bob imm imm_ppo. 
+Require Import imm. 
+Require Import imm_s. 
 Require Import FairExecution.
 From hahn Require Import Hahn.
+Require Import FinExecution.
 
 
-Definition imm_fair G := fsupp (⦗set_compl is_init⦘ ⨾ (ar G)⁺).
+Definition imm_fair G := fsupp (⦗set_compl is_init⦘ ⨾ (imm.ar G)⁺).
 Definition imm_s_fair G sc := fsupp (⦗set_compl is_init⦘ ⨾ (imm_s.ar G sc)⁺).
-
-
-Section ar_rf_ppo_sl_duplicate.
-  (* such lemmas exist for imm_s, but not for plain imm. *)
-  (* TODO: extract this and unify with existing code *)
-  Variables (G: execution).
-  Hypotheses (WF: Wf G).
-  Hypotheses (COM: complete G). 
-
-
-  Lemma IMM_ar_int_rfe_rf_ppo_loc_in_ar_int_rfe_ct :
-    (rfe G ∪ imm_ppo.ar_int G) ⨾ rf G ⨾ (ppo G ∩ same_loc (lab G)) ⊆ (rfe G ∪ imm_ppo.ar_int G)⁺.
-  Proof using WF.
-    remember (rfe G ∪ imm_ppo.ar_int G) as ax.
-    assert (sb G ⨾ sb G ⊆ sb G) as AA.
-    { apply transitiveI. apply sb_trans. }
-    
-    assert (rfi G ⨾ sb G ∩ same_loc (lab G) ⊆ sb G ∩ same_loc (lab G)) as DD.
-    { rewrite (rfi_in_sbloc' WF). apply transitiveI. apply sb_same_loc_trans. }
-    
-    rewrite rfi_union_rfe.
-    rewrite seq_union_l, seq_union_r.
-    unionL.
-    2: { arewrite (ppo G ∩ same_loc (lab G) ⊆ ppo G).
-         rewrite ppo_in_ar_int.
-         arewrite (rfe G ⨾ imm_ppo.ar_int G ⊆ ax  ⨾ ax).
-         { subst ax. basic_solver 10. }
-         arewrite (ax ⊆ ax⁺) at 1.
-         arewrite (ax ⊆ ax⁺) at 2. by rewrite ct_unit, ct_ct. }
-    subst ax.
-    rewrite !seq_union_l.
-    unionL.
-    { rewrite (dom_l (wf_rfiD WF)).
-      rewrite (dom_r (wf_rfeD WF)).
-      type_solver. }
-    unfold imm_ppo.ar_int at 1.
-    rewrite !seq_union_l.
-    unionL.
-    5: by rewrite (dom_l (wf_rfiD WF)); type_solver.
-    3: { rewrite (wf_detourD WF).
-         rewrite (wf_rfiD WF). type_solver. }
-    2: { arewrite (ppo G ∩ same_loc (lab G) ⊆ ppo G).
-         rewrite ppo_rfi_ppo. rewrite <- ct_step.
-         rewrite ppo_in_ar_int. eauto with hahn. }
-    2: { arewrite_id ⦗is_w (lab G)⦘ at 1. rewrite seq_id_l.
-         rewrite rfi_in_sb.
-         arewrite (ppo G ∩ same_loc (lab G) ⊆ ppo G).
-         rewrite (dom_r (@wf_ppoD G)).
-         rewrite (ppo_in_sb WF).
-         arewrite (sb G ⨾ sb G ⨾ sb G ⊆ sb G).
-         { generalize (@sb_trans G). basic_solver. }
-         rewrite <- ct_step.
-         rewrite w_ex_acq_sb_w_in_ar_int. eauto with hahn. }
-    rewrite (dom_r (@wf_ppoD G)).
-    rewrite (ppo_in_sb WF).
-    rewrite seq_eqv_inter_lr.
-    sin_rewrite DD.
-    rewrite bob_sb_same_loc_W_in_bob.
-    apply clos_trans_mori. rewrite bob_in_ar_int. eauto with hahn.
-  Qed.
-
-  Lemma IMM_ar_rf_ppo_loc_in_ar_ct :
-    ar G ⨾ rf G ⨾ ppo G ∩ same_loc (lab G) ⊆ (ar G)⁺.
-  Proof using WF.
-    unfold imm.ar.
-    rewrite unionA, seq_union_l.
-    unionL.
-    { rewrite wf_pscD, wf_rfD; auto. type_solver. }
-    rewrite IMM_ar_int_rfe_rf_ppo_loc_in_ar_int_rfe_ct.
-    apply clos_trans_mori. eauto with hahn.
-  Qed.
-
-  Lemma IMM_ar_ct_rf_ppo_loc_in_ar_ct :
-    (ar G)⁺ ⨾ rf G ⨾ ppo G ∩ same_loc (lab G) ⊆ (ar G)⁺.
-  Proof using WF.
-    rewrite ct_end at 1. rewrite !seqA.
-    rewrite IMM_ar_rf_ppo_loc_in_ar_ct.
-    apply rt_ct.
-  Qed.
-  
-  Lemma IMM_ar_ct_rf_ppo_loc_ct_in_ar_ct:
-    (ar G)⁺ ⨾ (rf G ⨾ ppo G ∩ same_loc (lab G))⁺ ⊆ (ar G)⁺.
-  Proof using WF.
-    intros x y [z [AA BB]].
-    apply clos_trans_t1n in BB.
-    induction BB.
-    2: apply IHBB.
-    all: apply IMM_ar_ct_rf_ppo_loc_in_ar_ct; auto.
-    all: eexists; split; eauto.
-  Qed.
-
-  Lemma IMM_ar_rf_ppo_loc_ct_in_ar_ct :
-    (ar G) ⨾ (rf G ⨾ ppo G ∩ same_loc (lab G))⁺ ⊆ (ar G)⁺.
-  Proof using WF.
-    rewrite ct_step with (r:=ar G) at 1.
-    by apply IMM_ar_ct_rf_ppo_loc_ct_in_ar_ct.
-  Qed.
-
-  Lemma IMM_ppo_loc_in_fr 
-        (SPL : sc_per_loc G) :
-    ppo G ∩ same_loc (lab G) ⊆ fr G.
-  Proof using WF COM.
-    rewrite wf_ppoD.
-    rewrite (ppo_in_sb WF).
-    rewrite seq_eqv_inter_ll.
-    rewrite seq_eqv_inter_lr.
-    rewrite r_sb_loc_w_in_fri; auto.
-    apply fri_in_fr.
-  Qed.
-  
-  Lemma IMM_ar_rf_ppo_loc_acyclic
-    (CONS: imm_consistent G):
-    acyclic (ar G ∪ rf G ⨾ ppo G ∩ same_loc (lab G)).
-  Proof using WF COM.
-    rewrite ct_step with (r:=ar G).
-    rewrite unionC.
-    apply acyclic_absorb.
-    { right. apply IMM_ar_ct_rf_ppo_loc_in_ar_ct. }
-    split.
-    2: { red. rewrite ct_of_ct. apply CONS. }
-    rewrite IMM_ppo_loc_in_fr; auto.
-    2: { apply coherence_sc_per_loc. by apply CONS. }
-    rewrite rf_fr; auto. by apply co_acyclic.
-  Qed.
-
-  Lemma IMM_no_ar_to_init : ar G ⨾ ⦗is_init⦘ ≡ ∅₂.
-  Proof using WF.
-    split; [|basic_solver].
-    unfold ar.
-    rewrite (ar_int_in_sb WF). rewrite no_sb_to_init.
-    rewrite wf_pscD. 
-    rewrite (wf_rfeD WF).
-    rewrite seq_union_l. unionL; [|basic_solver].
-    rewrite (init_w WF). type_solver 10.
-  Qed.
-
-  Lemma IMM_no_ar_rf_ppo_loc_to_init:
-    (ar G ∪ rf G ⨾ ppo G ∩ same_loc (lab G)) ⨾ ⦗is_init⦘ ≡ ∅₂.
-  Proof using WF.
-    split; [|basic_solver].
-    rewrite seq_union_l, seqA, IMM_no_ar_to_init; auto.
-    arewrite (ppo G ∩ same_loc (lab G) ⊆ ppo G).
-    rewrite (ppo_in_sb WF). rewrite no_sb_to_init.
-    basic_solver.
-  Qed.
-
-
-End ar_rf_ppo_sl_duplicate. 
 
 
 Section ImmFairProperties.
@@ -242,31 +95,26 @@ Section ImmFairProperties.
     2: { apply inclusion_ct_seq_eqv_l. } 
     apply clos_trans_mori. basic_solver. 
   Qed.
-
-  Lemma wf_ar_rf_ppo_loc_ct_inf_imm
-        (IMM_CONS: imm_consistent G)
-        (IMM_FAIR: imm_fair G):
-    well_founded (⦗set_compl is_init⦘ ⨾ (ar G ∪ rf G ;; ppo G ∩ same_loc (lab G))⁺).
-  Proof using WF FAIR COM.
-    apply wf_ar_rf_ppo_loc_ct_inf_helper; auto. 
-    { by apply IMM_ar_rf_ppo_loc_acyclic. }
-    { by apply IMM_no_ar_rf_ppo_loc_to_init. }
-    { by apply ppo_in_sb. }
-    { by apply IMM_ar_rf_ppo_loc_ct_in_ar_ct. }
-    cdes IMM_CONS. by apply coherence_sc_per_loc.
-  Qed. 
-    
-  Lemma wf_ar_rf_ppo_loc_ct_inf_imm_s
-        (IMM_CONS: imm_s.imm_consistent G sc)
-        (IMM_FAIR: imm_s_fair G sc):
-    well_founded (⦗set_compl is_init⦘ ⨾ (imm_s.ar G sc ∪ rf G ;; imm_s_ppo.ppo G ∩ same_loc (lab G))⁺).
-  Proof using WF FAIR COM.
-    apply wf_ar_rf_ppo_loc_ct_inf_helper; auto. 
-    { by apply ar_rf_ppo_loc_acyclic. }
-    { by apply no_ar_rf_ppo_loc_to_init. }
-    { by apply imm_s_ppo.ppo_in_sb. }
-    { by apply ar_rf_ppo_loc_ct_in_ar_ct. }
-    cdes IMM_CONS. by apply imm_s_hb.coherence_sc_per_loc.
-  Qed. 
-  
+      
 End ImmFairProperties.
+
+Lemma fin_exec_imm_s_fair G sc (WF: Wf G) (WFSC: wf_sc G sc)
+      (FIN: fin_exec G):
+  imm_s_fair G sc. 
+Proof. 
+  red. red in FIN.
+  eapply fsupp_mori.
+  2: { eapply fsupp_cross with (s' := set_full); eauto. }
+  red. rewrite ct_begin, wf_arE; auto. basic_solver.  
+Qed. 
+
+Lemma fin_exec_imm_fair G (WF: Wf G)
+      (FIN: fin_exec G):
+  imm_fair G. 
+Proof. 
+  red. red in FIN.
+  eapply fsupp_mori.
+  2: { eapply fsupp_cross with (s' := set_full); eauto. }
+  red. rewrite ct_begin, imm.wf_arE; auto. basic_solver.  
+Qed. 
+
