src/imm/imm_rfppo.v
@@ -1,0 +1,168 @@
+(* Require Import imm_s imm_s_ppo imm_s_hb.  *)
+Require Import Events.
+Require Import Execution.
+Require Import Execution_eco.
+Require Import imm_hb imm_bob imm imm_ppo. 
+From hahn Require Import Hahn.
+Require Import ImmFair.
+Require Import FairExecution. 
+
+
+Section ImmRfPpo.
+  (* TODO: unify with lemmas for imm_s *)
+  Variables (G: execution).
+  Hypotheses (WF: Wf G).
+  Hypotheses (COM: complete G). 
+
+
+  Lemma IMM_ar_int_rfe_rf_ppo_loc_in_ar_int_rfe_ct :
+    (rfe G ∪ imm_ppo.ar_int G) ⨾ rf G ⨾ (ppo G ∩ same_loc (lab G)) ⊆ (rfe G ∪ imm_ppo.ar_int G)⁺.
+  Proof using WF.
+    remember (rfe G ∪ imm_ppo.ar_int G) as ax.
+    assert (sb G ⨾ sb G ⊆ sb G) as AA.
+    { apply transitiveI. apply sb_trans. }
+    
+    assert (rfi G ⨾ sb G ∩ same_loc (lab G) ⊆ sb G ∩ same_loc (lab G)) as DD.
+    { rewrite (rfi_in_sbloc' WF). apply transitiveI. apply sb_same_loc_trans. }
+    
+    rewrite rfi_union_rfe.
+    rewrite seq_union_l, seq_union_r.
+    unionL.
+    2: { arewrite (ppo G ∩ same_loc (lab G) ⊆ ppo G).
+         rewrite ppo_in_ar_int.
+         arewrite (rfe G ⨾ imm_ppo.ar_int G ⊆ ax  ⨾ ax).
+         { subst ax. basic_solver 10. }
+         arewrite (ax ⊆ ax⁺) at 1.
+         arewrite (ax ⊆ ax⁺) at 2. by rewrite ct_unit, ct_ct. }
+    subst ax.
+    rewrite !seq_union_l.
+    unionL.
+    { rewrite (dom_l (wf_rfiD WF)).
+      rewrite (dom_r (wf_rfeD WF)).
+      type_solver. }
+    unfold imm_ppo.ar_int at 1.
+    rewrite !seq_union_l.
+    unionL.
+    5: by rewrite (dom_l (wf_rfiD WF)); type_solver.
+    3: { rewrite (wf_detourD WF).
+         rewrite (wf_rfiD WF). type_solver. }
+    2: { arewrite (ppo G ∩ same_loc (lab G) ⊆ ppo G).
+         rewrite ppo_rfi_ppo. rewrite <- ct_step.
+         rewrite ppo_in_ar_int. eauto with hahn. }
+    2: { arewrite_id ⦗is_w (lab G)⦘ at 1. rewrite seq_id_l.
+         rewrite rfi_in_sb.
+         arewrite (ppo G ∩ same_loc (lab G) ⊆ ppo G).
+         rewrite (dom_r (@wf_ppoD G)).
+         rewrite (ppo_in_sb WF).
+         arewrite (sb G ⨾ sb G ⨾ sb G ⊆ sb G).
+         { generalize (@sb_trans G). basic_solver. }
+         rewrite <- ct_step.
+         rewrite w_ex_acq_sb_w_in_ar_int. eauto with hahn. }
+    rewrite (dom_r (@wf_ppoD G)).
+    rewrite (ppo_in_sb WF).
+    rewrite seq_eqv_inter_lr.
+    sin_rewrite DD.
+    rewrite bob_sb_same_loc_W_in_bob.
+    apply clos_trans_mori. rewrite bob_in_ar_int. eauto with hahn.
+  Qed.
+
+  Lemma IMM_ar_rf_ppo_loc_in_ar_ct :
+    ar G ⨾ rf G ⨾ ppo G ∩ same_loc (lab G) ⊆ (ar G)⁺.
+  Proof using WF.
+    unfold imm.ar.
+    rewrite unionA, seq_union_l.
+    unionL.
+    { rewrite wf_pscD, wf_rfD; auto. type_solver. }
+    rewrite IMM_ar_int_rfe_rf_ppo_loc_in_ar_int_rfe_ct.
+    apply clos_trans_mori. eauto with hahn.
+  Qed.
+
+  Lemma IMM_ar_ct_rf_ppo_loc_in_ar_ct :
+    (ar G)⁺ ⨾ rf G ⨾ ppo G ∩ same_loc (lab G) ⊆ (ar G)⁺.
+  Proof using WF.
+    rewrite ct_end at 1. rewrite !seqA.
+    rewrite IMM_ar_rf_ppo_loc_in_ar_ct.
+    apply rt_ct.
+  Qed.
+  
+  Lemma IMM_ar_ct_rf_ppo_loc_ct_in_ar_ct:
+    (ar G)⁺ ⨾ (rf G ⨾ ppo G ∩ same_loc (lab G))⁺ ⊆ (ar G)⁺.
+  Proof using WF.
+    intros x y [z [AA BB]].
+    apply clos_trans_t1n in BB.
+    induction BB.
+    2: apply IHBB.
+    all: apply IMM_ar_ct_rf_ppo_loc_in_ar_ct; auto.
+    all: eexists; split; eauto.
+  Qed.
+
+  Lemma IMM_ar_rf_ppo_loc_ct_in_ar_ct :
+    (ar G) ⨾ (rf G ⨾ ppo G ∩ same_loc (lab G))⁺ ⊆ (ar G)⁺.
+  Proof using WF.
+    rewrite ct_step with (r:=ar G) at 1.
+    by apply IMM_ar_ct_rf_ppo_loc_ct_in_ar_ct.
+  Qed.
+
+  Lemma IMM_ppo_loc_in_fr 
+        (SPL : sc_per_loc G) :
+    ppo G ∩ same_loc (lab G) ⊆ fr G.
+  Proof using WF COM.
+    rewrite wf_ppoD.
+    rewrite (ppo_in_sb WF).
+    rewrite seq_eqv_inter_ll.
+    rewrite seq_eqv_inter_lr.
+    rewrite r_sb_loc_w_in_fri; auto.
+    apply fri_in_fr.
+  Qed.
+  
+  Lemma IMM_ar_rf_ppo_loc_acyclic
+    (CONS: imm_consistent G):
+    acyclic (ar G ∪ rf G ⨾ ppo G ∩ same_loc (lab G)).
+  Proof using WF COM.
+    rewrite ct_step with (r:=ar G).
+    rewrite unionC.
+    apply acyclic_absorb.
+    { right. apply IMM_ar_ct_rf_ppo_loc_in_ar_ct. }
+    split.
+    2: { red. rewrite ct_of_ct. apply CONS. }
+    rewrite IMM_ppo_loc_in_fr; auto.
+    2: { apply coherence_sc_per_loc. by apply CONS. }
+    rewrite rf_fr; auto. by apply co_acyclic.
+  Qed.
+
+  Lemma IMM_no_ar_to_init : ar G ⨾ ⦗is_init⦘ ≡ ∅₂.
+  Proof using WF.
+    split; [|basic_solver].
+    unfold ar.
+    rewrite (ar_int_in_sb WF). rewrite no_sb_to_init.
+    rewrite wf_pscD. 
+    rewrite (wf_rfeD WF).
+    rewrite seq_union_l. unionL; [|basic_solver].
+    rewrite (init_w WF). type_solver 10.
+  Qed.
+
+  Lemma IMM_no_ar_rf_ppo_loc_to_init:
+    (ar G ∪ rf G ⨾ ppo G ∩ same_loc (lab G)) ⨾ ⦗is_init⦘ ≡ ∅₂.
+  Proof using WF.
+    split; [|basic_solver].
+    rewrite seq_union_l, seqA, IMM_no_ar_to_init; auto.
+    arewrite (ppo G ∩ same_loc (lab G) ⊆ ppo G).
+    rewrite (ppo_in_sb WF). rewrite no_sb_to_init.
+    basic_solver.
+  Qed.
+
+  Lemma wf_ar_rf_ppo_loc_ct_inf_imm 
+        (IMM_CONS: imm_consistent G)
+        (IMM_FAIR: imm_fair G)
+        (FAIR: mem_fair G):
+    well_founded (⦗set_compl is_init⦘ ⨾ (ar G ∪ rf G ;; ppo G ∩ same_loc (lab G))⁺).
+  Proof using WF COM.
+    apply wf_ar_rf_ppo_loc_ct_inf_helper; auto. 
+    { by apply IMM_ar_rf_ppo_loc_acyclic. }
+    { by apply IMM_no_ar_rf_ppo_loc_to_init. }
+    { by apply ppo_in_sb. }
+    { by apply IMM_ar_rf_ppo_loc_ct_in_ar_ct. }
+    cdes IMM_CONS. by apply coherence_sc_per_loc.
+  Qed. 
+
+End ImmRfPpo. 
